module PLFA.P1-2-Induction where

import Relation.Binary.PropositionalEquality as Eq
open Eq using (_≡_; refl; cong; sym)
open Eq.≡-Reasoning using (begin_; step-≡-∣; step-≡-⟩; _∎)
open import Data.Nat using (ℕ; zero; suc; _+_; _*_; _∸_; _^_)

_ : (3 + 4) + 5 ≡ 3 + (4 + 5)
_ =
  begin
    (3 + 4) + 5
  ≡⟨⟩
    7 + 5
  ≡⟨⟩
    12
  ≡⟨⟩
    3 + 9
  ≡⟨⟩
    3 + (4 + 5)
  ∎

+-assoc : ∀ (m n p : ℕ) -> (m + n) + p ≡ m + (n + p)
+-assoc zero n p =
  begin
    (zero + n) + p
  ≡⟨⟩
    n + p
  ≡⟨⟩
    zero + (n + p)
  ∎
+-assoc (suc m) n p =
  begin
    (suc m + n) + p
  ≡⟨⟩
    suc (m + n) + p
  ≡⟨⟩
    suc ((m + n) + p)
  ≡⟨ cong suc (+-assoc m n p) ⟩
    suc (m + (n + p))
  ≡⟨⟩
    suc m + (n + p)
  ∎

+-identity : ∀ (m : ℕ) -> m + zero ≡ m
+-identity zero =
  begin
    zero + zero
  ≡⟨⟩
    zero
  ∎
+-identity (suc m) =
  begin
    suc m + zero
  ≡⟨⟩
    suc (m + zero)
  ≡⟨ cong suc (+-identity m) ⟩
    suc m
  ∎

+-suc : ∀ (m n : ℕ) -> m + suc n ≡ suc (m + n)
+-suc zero n =
  begin
    zero + suc n
  ≡⟨⟩
    suc n
  ≡⟨⟩
    suc (zero + n)
  ∎
+-suc (suc m) n =
  begin
    suc m + suc n
  ≡⟨⟩
    suc (m + suc n)
  ≡⟨ cong suc (+-suc m n) ⟩
    suc (suc (m + n))
  ≡⟨⟩
    suc (suc m + n)
  ∎

+-comm : ∀ (m n : ℕ) -> m + n ≡ n + m
+-comm m zero =
  begin
    m + zero
  ≡⟨ +-identity m ⟩
    m
  ≡⟨⟩
    zero + m
  ∎
+-comm m (suc n) =
  begin
    m + suc n
  ≡⟨ +-suc m n ⟩
    suc (m + n)
  ≡⟨ cong suc (+-comm m n) ⟩
    suc (n + m)
  ≡⟨⟩
    suc n + m
  ∎

+-rearrange : ∀ (m n p q : ℕ) -> (m + n) + (p + q) ≡ m + (n + p) + q
+-rearrange m n p q =
  begin
    (m + n) + (p + q)
  ≡⟨ sym (+-assoc (m + n) p q) ⟩
    ((m + n) + p) + q
  ≡⟨ cong (_+ q) (+-assoc m n p) ⟩
    (m + (n + p)) + q
  ≡⟨⟩
    m + (n + p) + q
  ∎

_ : (1 + 2) + 3 ≡ 1 + (2 + 3)
_ =
  begin
    (1 + 2) + 3
  ≡⟨⟩
    1 + (2 + 3)
  ∎

+-assoc' : ∀ (m n p : ℕ) -> (m + n) + p ≡ m + (n + p)
+-assoc' zero    n p = refl
+-assoc' (suc m) n p rewrite +-assoc' m n p = refl

+-identity' : ∀ (n : ℕ) -> n + zero ≡ n
+-identity' zero = refl
+-identity' (suc n) rewrite +-identity' n = refl

+-suc' : ∀ (m n : ℕ) -> m + suc n ≡ suc (m + n)
+-suc' zero n = refl
+-suc' (suc m) n rewrite +-suc' m n = refl

+-comm' : ∀ (m n : ℕ) -> m + n ≡ n + m
+-comm' m zero rewrite +-identity' m = refl
+-comm' m (suc n) rewrite +-suc' m n | +-comm' m n = refl

+-assoc'' : ∀ (m n p : ℕ) -> (m + n) + p ≡ m + (n + p)
+-assoc'' zero n p = refl
+-assoc'' (suc m) n p rewrite +-assoc'' m n p = refl

+-swap : ∀ (m n p : ℕ) -> (m + n) + p ≡ m + (n + p)
+-swap m n p =
  begin
    (m + n) + p
  ≡⟨ +-assoc m n p ⟩
    m + (n + p)
  ∎

*-distrib-+ : ∀ (m n p : ℕ) -> (m + n) * p ≡ m * p + n * p
*-distrib-+ zero n p =
  begin
    (zero + n) * p
  ≡⟨⟩
    n * p
  ≡⟨⟩
    zero + n * p
  ≡⟨⟩
    zero * p + n * p
  ∎
*-distrib-+ (suc m) n p =
  begin
    (suc m + n) * p
  ≡⟨⟩
    suc (m + n) * p
  ≡⟨⟩
    p + (m + n) * p
  ≡⟨ cong (p +_) (*-distrib-+ m n p) ⟩
    p + (m * p + n * p)
  ≡⟨ sym (+-assoc p (m * p) (n * p)) ⟩
    (p + m * p) + n * p
  ≡⟨⟩
    suc m * p + n * p
  ∎

*-assoc : ∀ (m n p : ℕ) -> (m * n) * p ≡ m * (n * p)
*-assoc zero n p =
  begin
    (zero * n) * p
  ≡⟨⟩
    zero * p
  ≡⟨⟩
    zero * (n * p)
  ∎
*-assoc (suc m) n p =
  begin
    (suc m * n) * p
  ≡⟨⟩
    (n + (m * n)) * p
  ≡⟨ *-distrib-+ n (m * n) p ⟩
    (n * p) + (m * n) * p
  ≡⟨ cong ((n * p) +_) (*-assoc m n p) ⟩
    (n * p) + m * (n * p)
  ≡⟨⟩
    (suc zero + m) * (n * p)
  ≡⟨⟩
    suc m * (n * p)
  ∎

*-identity : ∀ (m : ℕ) -> m * suc zero ≡ m
*-identity zero =
  begin
    zero * suc zero
  ≡⟨⟩
    zero
  ∎
*-identity (suc m) =
  begin
    suc m * suc zero
  ≡⟨⟩
    suc (m * suc zero)
  ≡⟨ cong suc (*-identity m) ⟩
    suc m
  ∎

_ : 1 * 0 ≡ 0
_ =
  begin
    1 * 0
  ≡⟨⟩
    0
  ∎

*-zero : ∀ (n : ℕ) -> n * zero ≡ zero
*-zero zero = refl
*-zero (suc n) rewrite *-zero n = refl

*-comm : ∀ (m n : ℕ) -> m * n ≡ n * m
*-comm m zero =
  begin
    m * zero
  ≡⟨ *-zero m ⟩
    zero
  ≡⟨⟩
    zero * m
  ∎
*-comm m (suc n) =
  begin
    m * suc n
  ≡⟨⟩
    ?
  ≡⟨⟩
    suc n * m
  ∎
